boringssl_fips_20180730/spec_digest_base.v
@@ -1,6 +1,111 @@
 Require Export VST.floyd.proofauto.
 Require Import boringssl_fips_20180730.digests.
+Require Import boringssl_fips_20180730.spec_mem. (*needed (only) for parameters WA and WORD*)
 Require Export boringssl_fips_20180730.digest_model.
+
+(*General lemmas, to be moved elsewhere*)
+Lemma Valeq_Vint {A} i j (a b:A):
+      (if Val.eq (Vint i) (Vint j) then a else b) =
+      (if Int.eq i j then a else b).
+Proof. 
+ remember (Int.eq i j). destruct b0.
++ rewrite ( binop_lemmas2.int_eq_true _ _ Heqb0). rewrite if_true; trivial.
++ remember (Val.eq (Vint i )(Vint j)) as d.
+  destruct d; trivial.
+  inversion e; subst; simpl in *.
+  specialize (int_eq_false_e j j); intuition.
+Qed. 
+
+Lemma ptr_comp_Cne_t p q (P: is_pointer_or_null p) (Q: is_pointer_or_null q): 
+      typed_true tint (force_val (sem_cmp_pp Cne p q)) <-> ~(p=q).
+Proof.
+  destruct p; destruct q; try contradiction; simpl in *; subst;
+  unfold typed_true, sem_cmp_pp; simpl; split; intros; trivial; try solve [inv H].
++ elim H; trivial.
++ intros N; inv N. rewrite if_true, Ptrofs.eq_true in H; trivial; inv H.
++ destruct (eq_block b b0); subst; trivial.
+  destruct (Ptrofs.eq_dec i i0); subst; [ elim H; trivial | rewrite Ptrofs.eq_false; trivial].
+Qed.
+
+Lemma ptr_comp_Cne_t' {T} p q 
+      (H: typed_true tint (force_val (sem_cmp_pp Cne p q)))
+       (a b:T) (P: is_pointer_or_null p)
+               (Q: is_pointer_or_null q):
+      (if Val.eq p q then a else b) = b.
+Proof. apply ptr_comp_Cne_t in H; trivial.
+  rewrite if_false; trivial.
+Qed.
+
+Lemma ptr_comp_Cne_f p q (P: is_pointer_or_null p) (Q: is_pointer_or_null q): 
+      typed_false tint (force_val (sem_cmp_pp Cne p q)) <-> (p=q).
+Proof.
+  destruct p; destruct q; try contradiction; simpl in *; subst;
+  unfold typed_false, sem_cmp_pp; simpl; split; intros; trivial; try solve [inv H].
++ destruct (eq_block b b0); [subst; simpl in H | inv H].
+  destruct (Ptrofs.eq_dec i i0); subst; trivial.
+  rewrite Ptrofs.eq_false in H; trivial; inv H. 
++ inv H. rewrite if_true, Ptrofs.eq_true; trivial. 
+Qed.
+
+Lemma ptr_comp_Cne_f' {T} p q 
+      (H: typed_false tint (force_val (sem_cmp_pp Cne p q)))
+       (a b:T) (P: is_pointer_or_null p)
+               (Q: is_pointer_or_null q):
+      (if Val.eq p q then a else b) = a.
+Proof. apply ptr_comp_Cne_f in H; trivial.
+  rewrite if_true; trivial.
+Qed.
+
+Lemma data_at__valid_pointer {cs : compspecs} sh t p:
+  sepalg.nonidentity sh ->
+  sizeof t > 0 ->
+  @data_at_ cs sh t p |-- valid_pointer p.
+Proof. intros. unfold data_at_, field_at_. apply field_at_valid_ptr0; simpl; trivial. Qed.
+
+Lemma func_ptr'_isptr' v f: (func_ptr' f v) = ((!! isptr v) && func_ptr' f v).
+Proof. apply pred_ext; entailer!. Qed.
+
+Lemma writable_nonidentity sh (W:writable_share sh): sepalg.nonidentity sh.
+Proof. apply readable_nonidentity. apply writable_readable; trivial. Qed.
+
+Lemma semax_orp {cs Espec Delta P1 P2 Q c}
+  (HR1: @semax cs Espec Delta P1 c Q)
+  (HR2: @semax cs Espec Delta P2 c Q):
+  @semax cs Espec Delta (P1 || P2) c Q.
+Proof.
+ eapply semax_pre with (P':=EX x:bool, if x then P1 else P2).
++ old_go_lower. apply orp_left; [Exists true | Exists false]; entailer!.
++ Intros b. destruct b; trivial.
+Qed.
+
+Lemma semax_orp_SEPx (cs : compspecs) (Espec : OracleKind)
+      (Delta : tycontext) (P : list Prop) (Q : list localdef)
+      (R1 R2 : mpred) (R:list mpred) (T : ret_assert) (c : statement)
+  (HR1 : semax Delta
+         (PROPx P (LOCALx Q (SEPx (cons R1 R)))) c T)
+  (HR2 : semax Delta
+         (PROPx P (LOCALx Q (SEPx (cons R2 R)))) c T):
+semax Delta
+  (PROPx P (LOCALx Q (SEPx (cons (orp R1 R2) R)))) c T.
+Proof.
+ eapply semax_pre; [| apply (semax_orp HR1 HR2)].
+ old_go_lower.
+ rewrite distrib_orp_sepcon. normalize. 
+Qed.
+
+Lemma semax_orp_SEPnil cs Espec Delta P Q R1 R2 T c
+  (HR1: @semax cs Espec Delta (PROP (P) LOCAL (Q) SEP (R1)) c T)
+  (HR2: @semax cs Espec Delta (PROP (P) LOCAL (Q) SEP (R2)) c T):
+  @semax cs Espec Delta (PROP (P) LOCAL (Q) SEP (R1 || R2)) c T.
+Proof. apply semax_orp_SEPx; trivial. Qed.
+Lemma semax_orp_SEP cs Espec Delta P Q R1 R2 R T c
+  (HR1: @semax cs Espec Delta (PROP (P) LOCAL (Q) SEP (R1; R)) c T)
+  (HR2: @semax cs Espec Delta (PROP (P) LOCAL (Q) SEP (R2; R)) c T):
+  @semax cs Espec Delta (PROP (P) LOCAL (Q) SEP ((R1 || R2); R)) c T.
+Proof. apply semax_orp_SEPx; trivial. Qed.
+
+(**************************************)
+
 
 Require Export sha.vst_lemmas. (*for definition of data_block. *)
 
@@ -13,6 +118,8 @@ Record MD_with_content :=
     __content : mddataTp __EVP_MD
   }.
 
+Parameter rep: MD_with_content -> list byte -> Prop.
+
 (*The generalization of sha's predicate sha256state_ to other digest functions*)
 (*TDOD: replace by
   Definition MD_state (sh:share) (DC: MD_with_content):  val -> mpred :=
@@ -21,9 +128,19 @@ Record MD_with_content :=
   | _ => fun p => FF (*TODO: replace by suitable predicates for other digests*)
   end.*)
 
-Parameter MD_state: forall (sh:share) (DC: MD_with_content), val -> mpred.
-Parameter MD_state_memoryblock: forall sh DC p,
+Definition MD_state (sh:share) (DC: MD_with_content) (v:val): mpred :=
+  EX contents: list byte, 
+  !!(Zlength contents = (ctx_size_of_MD (__EVP_MD DC)) /\
+     rep DC contents) &&
+  data_block sh contents v.
+
+Lemma MD_state_memoryblock sh DC p:
       MD_state sh DC p |-- memory_block sh (ctx_size_of_MD (__EVP_MD DC)) p.
+Proof. unfold MD_state, data_block; Intros c. rewrite H.
+  eapply derives_trans. apply data_at_memory_block.
+  specialize (Zlength_nonneg c); intros.
+  simpl. rewrite Z.mul_1_l, Z.max_r; trivial; omega.
+Qed.
 
 (******* Access functions for reptype (Tstruct _env_md_ctx_st noattr) **)
 
@@ -104,15 +221,25 @@ Definition update_spec (D:EVP_MD):funspec :=
           SEP(data_at sh (Tstruct _env_md_ctx_st noattr) CTX ctx;
               data_block dsh data d;
               MD_state mdsh (UPD DC data len) (mddata_of_ctx CTX)).
+(*
+Definition postFin sh (n:Z) p: mpred := EX bytes:list byte, 
+           !!(0 <= n) && (*data_at sh (tarray tuchar n) (list_repeat (Z.to_nat n) (Vubyte Byte.zero)) p*)
+                data_at sh (tarray tuchar n) (map Vubyte bytes) p.*)
+Definition postFin sh D p: mpred := 
+(*  EX c:_, MD_state sh (Build_MD_with_content D c) p.*)
+  EX contents: list byte, 
+  !!(Zlength contents = (ctx_size_of_MD D)(* /\
+     rep DC contents*)) &&
+  data_block sh contents p.
 
-Definition postFin sh (n:Z) p: mpred :=
-           !!(0 <= n) && data_at sh (tarray tuchar n) (list_repeat (Z.to_nat n) (Vint Int.zero)) p.
-Lemma postFin_memory_block sh n p: postFin sh n p |-- memory_block sh n p.
-Proof. unfold postFin; Intros. eapply derives_trans. apply data_at_memory_block.
-  simpl. rewrite Z.mul_1_l, Z.max_r; trivial.
+Lemma postFin_memory_block sh D p: postFin sh D p |-- memory_block sh (ctx_size_of_MD D) p.
+Proof. unfold postFin. Intros bytes.
+  eapply derives_trans. apply data_at_memory_block.
+  simpl in *. rewrite Z.mul_1_l, Z.max_r, H; trivial.
+  apply Zlength_nonneg.
 Qed.
  
-Lemma postFin_pTN sh n md: postFin sh n md |-- !!(is_pointer_or_null md).
+Lemma postFin_pTN sh D md: postFin sh D md |-- !!(is_pointer_or_null md).
 Proof. eapply derives_trans. apply postFin_memory_block. entailer!. Qed.
 
 Definition FinalSideconditions (DC: MD_with_content) (len:Z) : Prop :=
@@ -136,15 +263,27 @@ Definition final_spec (D:EVP_MD): funspec :=
   POST [ tvoid ]
           PROP() LOCAL () 
           SEP(data_at sh (Tstruct _env_md_ctx_st noattr) CTX ctx;
-              postFin mdsh (ctx_size_of_MD (__EVP_MD DC)) (mddata_of_ctx CTX);
+              postFin mdsh (__EVP_MD DC) (mddata_of_ctx CTX);
               data_block osh (FIN DC) out).
-
+(*
 Parameter preInit: share -> Z -> val -> mpred.
 (*Parameter preInit_fresh: forall sh sz m, 
   memory_block Tsh sz m |--preInit sh sz m. *)(*Presumably, we'll only permit sh==Tsh because of this*)
 
 Parameter preInit_fresh_EWS: forall sz m, 
   memory_block Ews sz m |--preInit Ews sz m.
+*)
+
+Definition preInit sh n p: mpred := 
+  !!(0 <= n) && data_at_ sh (tarray tuchar n) p.
+Lemma preInit_fresh_EWS sz m (H:0 <= sz < Ptrofs.modulus):
+  memory_block Ews sz m |--preInit Ews sz m.
+Proof. unfold preInit. entailer!. eapply memory_block_data_at__tarray_tuchar; trivial.
+Qed.
+
+Lemma postFin_preInit sh D m: postFin sh D m |-- preInit sh (ctx_size_of_MD D) m.
+Proof. unfold postFin, preInit, MD_state. Intros c.
+  simpl in *. unfold data_block. rewrite H; entailer!. Qed.
 
 Definition INI (D: EVP_MD): MD_with_content :=
   let cont := EVP_MD_rec_init _ (EVPMD_record_of_EVPMD D)
@@ -200,12 +339,10 @@ Definition match_EVP_MD (D:EVP_MD) (vals: reptype (Tstruct _env_md_st noattr)): 
        func_ptr' (final_spec D) fin)
   end.
 
-
 Definition EVP_MD_rep (D:EVP_MD) (p:val):mpred :=
   EX sh:_, EX vals :_,
-  !!(readable_share sh) && match_EVP_MD D vals *
+  !!(readable_share sh /\ 4 <= (ctx_size_of_MD D) <= Int.max_unsigned - (WA + WORD) - 8) && match_EVP_MD D vals *
   (data_at sh (Tstruct _env_md_st noattr) vals p).
-
 
 (**************** Lemmas about these constructions *********************)
 
@@ -217,3 +354,10 @@ Proof. apply pred_ext; entailer. apply EVP_MD_rep_isptr. Qed.
 
 Lemma EVP_MD_rep_validptr R p:  EVP_MD_rep R p |-- valid_pointer p.
 Proof. unfold EVP_MD_rep. Intros sh vals. entailer!. Qed.
+
+Lemma match_EVP_MD_getctxsize D dvals : match_EVP_MD D dvals |-- !!(get_ctxsize dvals = Vint (Int.repr (ctx_size_of_MD D))).
+Proof. unfold match_EVP_MD. destruct dvals as [type [mds [flags [ini [upd [fin [blsize ctxsize]]]]]]]. simpl in *. entailer!. Qed.
+
+Lemma match_EVP_MD_getctxsize' D dvals : match_EVP_MD D dvals =
+      (!!(get_ctxsize dvals = Vint (Int.repr (ctx_size_of_MD D))) && match_EVP_MD D dvals).
+Proof. apply pred_ext; entailer; apply match_EVP_MD_getctxsize. Qed.
