boringssl_fips_20180730/vstlib.v
@@ -1,0 +1,101 @@
+Require Import VST.floyd.proofauto.
+
+Lemma Valeq_Vint {A} i j (a b:A):
+      (if Val.eq (Vint i) (Vint j) then a else b) =
+      (if Int.eq i j then a else b).
+Proof. 
+ remember (Int.eq i j). destruct b0.
++ rewrite ( binop_lemmas2.int_eq_true _ _ Heqb0). rewrite if_true; trivial.
++ remember (Val.eq (Vint i )(Vint j)) as d.
+  destruct d; trivial.
+  inversion e; subst; simpl in *.
+  specialize (int_eq_false_e j j); intuition.
+Qed. 
+
+Lemma ptr_comp_Cne_t p q (P: is_pointer_or_null p) (Q: is_pointer_or_null q): 
+      typed_true tint (force_val (sem_cmp_pp Cne p q)) <-> ~(p=q).
+Proof.
+  destruct p; destruct q; try contradiction; simpl in *; subst;
+  unfold typed_true, sem_cmp_pp; simpl; split; intros; trivial; try solve [inv H]; try discriminate.
++ elim H; trivial.
++ intros N; inv N. rewrite if_true, Ptrofs.eq_true in H; trivial; inv H.
++ destruct (eq_block b b0); subst; trivial.
+  destruct (Ptrofs.eq_dec i i0); subst; [ elim H; trivial | rewrite Ptrofs.eq_false; trivial].
+Qed.
+
+Lemma ptr_comp_Cne_t' {T} p q 
+      (H: typed_true tint (force_val (sem_cmp_pp Cne p q)))
+       (a b:T) (P: is_pointer_or_null p)
+               (Q: is_pointer_or_null q):
+      (if Val.eq p q then a else b) = b.
+Proof. apply ptr_comp_Cne_t in H; trivial.
+  rewrite if_false; trivial.
+Qed.
+
+Lemma ptr_comp_Cne_f p q (P: is_pointer_or_null p) (Q: is_pointer_or_null q): 
+      typed_false tint (force_val (sem_cmp_pp Cne p q)) <-> (p=q).
+Proof.
+  destruct p; destruct q; try contradiction; simpl in *; subst;
+  unfold typed_false, sem_cmp_pp; simpl; split; intros; trivial; try solve [inv H].
++ destruct (eq_block b b0); [subst; simpl in H | inv H].
+  destruct (Ptrofs.eq_dec i i0); subst; trivial.
+  rewrite Ptrofs.eq_false in H; trivial; inv H. 
++ inv H. rewrite if_true, Ptrofs.eq_true; trivial. 
+Qed.
+
+Lemma ptr_comp_Cne_f' {T} p q 
+      (H: typed_false tint (force_val (sem_cmp_pp Cne p q)))
+       (a b:T) (P: is_pointer_or_null p)
+               (Q: is_pointer_or_null q):
+      (if Val.eq p q then a else b) = a.
+Proof. apply ptr_comp_Cne_f in H; trivial.
+  rewrite if_true; trivial.
+Qed.
+
+Lemma data_at__valid_pointer {cs : compspecs} sh t p:
+  sepalg.nonidentity sh ->
+  sizeof t > 0 ->
+  @data_at_ cs sh t p |-- valid_pointer p.
+Proof. intros. unfold data_at_, field_at_. apply field_at_valid_ptr0; simpl; trivial. Qed.
+
+Lemma func_ptr'_isptr' v f: (func_ptr' f v) = ((!! isptr v) && func_ptr' f v).
+Proof. apply pred_ext; entailer!. Qed.
+
+Lemma writable_nonidentity sh (W:writable_share sh): sepalg.nonidentity sh.
+Proof. apply readable_nonidentity. apply writable_readable; trivial. Qed.
+
+Lemma semax_orp {cs Espec Delta P1 P2 Q c}
+  (HR1: @semax cs Espec Delta P1 c Q)
+  (HR2: @semax cs Espec Delta P2 c Q):
+  @semax cs Espec Delta (P1 || P2) c Q.
+Proof.
+ eapply semax_pre with (P':=EX x:bool, if x then P1 else P2).
++ old_go_lower. apply orp_left; [Exists true | Exists false]; entailer!.
++ Intros b. destruct b; trivial.
+Qed.
+
+Lemma semax_orp_SEPx (cs : compspecs) (Espec : OracleKind)
+      (Delta : tycontext) (P : list Prop) (Q : list localdef)
+      (R1 R2 : mpred) (R:list mpred) (T : ret_assert) (c : statement)
+  (HR1 : semax Delta
+         (PROPx P (LOCALx Q (SEPx (cons R1 R)))) c T)
+  (HR2 : semax Delta
+         (PROPx P (LOCALx Q (SEPx (cons R2 R)))) c T):
+semax Delta
+  (PROPx P (LOCALx Q (SEPx (cons (orp R1 R2) R)))) c T.
+Proof.
+ eapply semax_pre; [| apply (semax_orp HR1 HR2)].
+ old_go_lower.
+ rewrite distrib_orp_sepcon. normalize. 
+Qed.
+
+Lemma semax_orp_SEPnil cs Espec Delta P Q R1 R2 T c
+  (HR1: @semax cs Espec Delta (PROP (P) LOCAL (Q) SEP (R1)) c T)
+  (HR2: @semax cs Espec Delta (PROP (P) LOCAL (Q) SEP (R2)) c T):
+  @semax cs Espec Delta (PROP (P) LOCAL (Q) SEP (R1 || R2)) c T.
+Proof. apply semax_orp_SEPx; trivial. Qed.
+Lemma semax_orp_SEP cs Espec Delta P Q R1 R2 R T c
+  (HR1: @semax cs Espec Delta (PROP (P) LOCAL (Q) SEP (R1; R)) c T)
+  (HR2: @semax cs Espec Delta (PROP (P) LOCAL (Q) SEP (R2; R)) c T):
+  @semax cs Espec Delta (PROP (P) LOCAL (Q) SEP ((R1 || R2); R)) c T.
+Proof. apply semax_orp_SEPx; trivial. Qed.
